misc/treiber-known.bpl
@@ -4,31 +4,31 @@
 // known() trick to control instantiations.
 // ----------------------------------------
 
-type Loc;
-const null: Loc;
+type Ref;
+const null: Ref;
 
 type Heap;
-function {:linear "Node"} dom(Heap): [Loc]bool;
-function next(Heap): [Loc]Loc;
-function {:builtin "MapConst"} MapConstBool(bool) : [Loc]bool;
+function {:linear "Node"} dom(Heap): [Ref]bool;
+function next(Heap): [Ref]Ref;
+function {:builtin "MapConst"} MapConstBool(bool) : [Ref]bool;
 
 function EmptyHeap(): (Heap);
 axiom (dom(EmptyHeap()) == MapConstBool(false));
 
-function Add(h: Heap, l: Loc, v: Loc): (Heap);
-axiom (forall h: Heap, l: Loc, v: Loc :: dom(Add(h, l, v)) == dom(h)[l:=true] && next(Add(h, l, v)) == next(h)[l := v]);
+function Add(h: Heap, l: Ref, v: Ref): (Heap);
+axiom (forall h: Heap, l: Ref, v: Ref :: dom(Add(h, l, v)) == dom(h)[l:=true] && next(Add(h, l, v)) == next(h)[l := v]);
 
-function Remove(h: Heap, l: Loc): (Heap);
-axiom (forall h: Heap, l: Loc :: dom(Remove(h, l)) == dom(h)[l:=false] && next(Remove(h, l)) == next(h));
+function Remove(h: Heap, l: Ref): (Heap);
+axiom (forall h: Heap, l: Ref :: dom(Remove(h, l)) == dom(h)[l:=false] && next(Remove(h, l)) == next(h));
 
 // Linearity stuff:
 
 // TODO is this one ever used?
-function {:inline} {:linear "Node"} NodeCollector(x: Loc) : [Loc]bool
+function {:inline} {:linear "Node"} NodeCollector(x: Ref) : [Ref]bool
 {
   MapConstBool(false)[x := true]
 }
-function {:inline} {:linear "Node"} NodeSetCollector(x: [Loc]bool) : [Loc]bool
+function {:inline} {:linear "Node"} NodeSetCollector(x: [Ref]bool) : [Ref]bool
 {
   x
 }
@@ -37,82 +37,82 @@ function {:inline} {:linear "Node"} NodeSetCollector(x: [Loc]bool) : [Loc]bool
 // ---------- Reachability, between, and associated theories
 
 // Predicates used to control the triggers on the below axioms
-function known(x: Loc) : bool;
-function knownF(f: [Loc]Loc) : bool;
-axiom(forall x: Loc :: {known(x)} known(x));
-axiom(forall f: [Loc]Loc :: {knownF(f)} knownF(f));
+function known(x: Ref) : bool;
+function knownF(f: [Ref]Ref) : bool;
+axiom(forall x: Ref :: {known(x)} known(x));
+axiom(forall f: [Ref]Ref :: {knownF(f)} knownF(f));
 
  
 ////////////////////
 // Between predicate
 ////////////////////
-function Between(f: [Loc]Loc, x: Loc, y: Loc, z: Loc) returns (bool);
-function Avoiding(f: [Loc]Loc, x: Loc, y: Loc, z: Loc) returns (bool);
+function Btwn(f: [Ref]Ref, x: Ref, y: Ref, z: Ref) returns (bool);
+function ReachW(f: [Ref]Ref, x: Ref, y: Ref, z: Ref) returns (bool);
 
 
 //////////////////////////
-// Axioms for Between
+// Axioms for Btwn
 //////////////////////////
 
 // read null
-axiom (forall f: [Loc]Loc :: f[null] == null);
+axiom (forall f: [Ref]Ref :: f[null] == null);
 
 // reflexive
-axiom(forall f: [Loc]Loc, x: Loc :: Between(f, x, x, x));
+axiom(forall f: [Ref]Ref, x: Ref :: Btwn(f, x, x, x));
 
 // step
-axiom(forall f: [Loc]Loc, x: Loc :: {f[x]} Between(f, x, f[x], f[x]));
+axiom(forall f: [Ref]Ref, x: Ref :: {f[x]} Btwn(f, x, f[x], f[x]));
 
 // reach
-axiom(forall f: [Loc]Loc, x: Loc, y: Loc :: {f[x], known(y)} Between(f, x, y, y) ==> x == y || Between(f, x, f[x], y));
+axiom(forall f: [Ref]Ref, x: Ref, y: Ref :: {f[x], known(y)} Btwn(f, x, y, y) ==> x == y || Btwn(f, x, f[x], y));
 
 // cycle
-axiom(forall f: [Loc]Loc, x: Loc, y:Loc :: {f[x], known(y)} f[x] == x && Between(f, x, y, y) ==> x == y);
+axiom(forall f: [Ref]Ref, x: Ref, y:Ref :: {f[x], known(y)} f[x] == x && Btwn(f, x, y, y) ==> x == y);
 
 // sandwich
-axiom(forall f: [Loc]Loc, x: Loc, y: Loc :: {knownF(f), known(x), known(y), Between(f, x, y, x)} Between(f, x, y, x) ==> x == y);
+axiom(forall f: [Ref]Ref, x: Ref, y: Ref :: {knownF(f), known(x), known(y), Btwn(f, x, y, x)} Btwn(f, x, y, x) ==> x == y);
 
 // order1
-axiom(forall f: [Loc]Loc, x: Loc, y: Loc, z: Loc :: {knownF(f), known(x), known(y), known(z), Between(f, x, y, y), Between(f, x, z, z)} Between(f, x, y, y) && Between(f, x, z, z) ==> Between(f, x, y, z) || Between(f, x, z, y));
+axiom(forall f: [Ref]Ref, x: Ref, y: Ref, z: Ref :: {knownF(f), known(x), known(y), known(z), Btwn(f, x, y, y), Btwn(f, x, z, z)} Btwn(f, x, y, y) && Btwn(f, x, z, z) ==> Btwn(f, x, y, z) || Btwn(f, x, z, y));
 
 // order2
-axiom(forall f: [Loc]Loc, x: Loc, y: Loc, z: Loc :: {knownF(f), known(x), known(y), known(z), Between(f, x, y, z)} Between(f, x, y, z) ==> Between(f, x, y, y) && Between(f, y, z, z));
+axiom(forall f: [Ref]Ref, x: Ref, y: Ref, z: Ref :: {knownF(f), known(x), known(y), known(z), Btwn(f, x, y, z)} Btwn(f, x, y, z) ==> Btwn(f, x, y, y) && Btwn(f, y, z, z));
 
 // transitive1
-axiom(forall f: [Loc]Loc, x: Loc, y: Loc, z: Loc :: {knownF(f), known(x), known(y), known(z), Between(f, x, y, y), Between(f, y, z, z)} Between(f, x, y, y) && Between(f, y, z, z) ==> Between(f, x, z, z));
+axiom(forall f: [Ref]Ref, x: Ref, y: Ref, z: Ref :: {knownF(f), known(x), known(y), known(z), Btwn(f, x, y, y), Btwn(f, y, z, z)} Btwn(f, x, y, y) && Btwn(f, y, z, z) ==> Btwn(f, x, z, z));
 
 // transitive2
-axiom(forall f: [Loc]Loc, x: Loc, y: Loc, z: Loc, w: Loc :: {knownF(f), known(x), known(y), known(z), known(w), Between(f, x, y, z), Between(f, y, w, z)} Between(f, x, y, z) && Between(f, y, w, z) ==> Between(f, x, y, w) && Between(f, x, w, z));
+axiom(forall f: [Ref]Ref, x: Ref, y: Ref, z: Ref, w: Ref :: {knownF(f), known(x), known(y), known(z), known(w), Btwn(f, x, y, z), Btwn(f, y, w, z)} Btwn(f, x, y, z) && Btwn(f, y, w, z) ==> Btwn(f, x, y, w) && Btwn(f, x, w, z));
 
 // transitive3
-axiom(forall f: [Loc]Loc, x: Loc, y: Loc, z: Loc, w: Loc :: {knownF(f), known(x), known(y), known(z), known(w), Between(f, x, y, z), Between(f, x, w, y)} Between(f, x, y, z) && Between(f, x, w, y) ==> Between(f, x, w, z) && Between(f, w, y, z));
+axiom(forall f: [Ref]Ref, x: Ref, y: Ref, z: Ref, w: Ref :: {knownF(f), known(x), known(y), known(z), known(w), Btwn(f, x, y, z), Btwn(f, x, w, y)} Btwn(f, x, y, z) && Btwn(f, x, w, y) ==> Btwn(f, x, w, z) && Btwn(f, w, y, z));
 
-// relation between Avoiding and Between
-axiom(forall f: [Loc]Loc, x: Loc, y: Loc, z: Loc :: {knownF(f), known(x), known(y), known(z), Avoiding(f, x, y, z)} Avoiding(f, x, y, z) <==> (Between(f, x, y, z) || (Between(f, x, y, y) && !Between(f, x, z, z))));
-axiom(forall f: [Loc]Loc, x: Loc, y: Loc, z: Loc :: {knownF(f), known(x), known(y), known(z), Between(f, x, y, z)} Between(f, x, y, z) <==> (Avoiding(f, x, y, z) && Avoiding(f, x, z, z)));
+// relation between ReachW and Btwn
+axiom(forall f: [Ref]Ref, x: Ref, y: Ref, z: Ref :: {knownF(f), known(x), known(y), known(z), ReachW(f, x, y, z)} ReachW(f, x, y, z) <==> (Btwn(f, x, y, z) || (Btwn(f, x, y, y) && !Btwn(f, x, z, z))));
+axiom(forall f: [Ref]Ref, x: Ref, y: Ref, z: Ref :: {knownF(f), known(x), known(y), known(z), Btwn(f, x, y, z)} Btwn(f, x, y, z) <==> (ReachW(f, x, y, z) && ReachW(f, x, z, z)));
 
 // btwn_write: grasshopper's update axiom
-axiom (forall f: [Loc]Loc, x: Loc, y: Loc, z: Loc, u: Loc, v: Loc :: {f[u := v], known(x), known(y), known(z), Between(f[u := v], x, y, z)}
+axiom (forall f: [Ref]Ref, x: Ref, y: Ref, z: Ref, u: Ref, v: Ref :: {f[u := v], known(x), known(y), known(z), Btwn(f[u := v], x, y, z)}
         u != null ==>
-          (Between(f[u := v], x, y, z) <==>
-          (Between(f, x, y, z) && Avoiding(f, x, z, u))
-          || (u != z && Avoiding(f, x, u, z) && Avoiding(f, v, z, u)
-            && (Between(f, x, y, u) || Between(f, v, y, z)))));
+          (Btwn(f[u := v], x, y, z) <==>
+          (Btwn(f, x, y, z) && ReachW(f, x, z, u))
+          || (u != z && ReachW(f, x, u, z) && ReachW(f, v, z, u)
+            && (Btwn(f, x, y, u) || Btwn(f, v, y, z)))));
 
 
 // ---------- Shared state and invariant
 
 var {:linear "Node"} {:layer 0,2} Stack: Heap;
-var {:linear "Node"} {:layer 0,2} Used: [Loc]bool;
+var {:linear "Node"} {:layer 0,2} Used: [Ref]bool;
 
-var {:layer 0,2} TopOfStack: Loc;
+var {:layer 0,2} TopOfStack: Ref;
 
 
-function {:inline} Inv(TopOfStack: Loc, Stack: Heap) : (bool)
+function {:inline} Inv(TopOfStack: Ref, Stack: Heap) : (bool)
 {
-  Between(next(Stack), TopOfStack, TopOfStack, null)
-    && (forall l: Loc :: {Between(next(Stack), TopOfStack, l, null)} known(l) ==>
-       (Between(next(Stack), TopOfStack, l, null)
+  Btwn(next(Stack), TopOfStack, TopOfStack, null)
+    && (forall l: Ref :: {Btwn(next(Stack), TopOfStack, l, null)} known(l) ==>
+       (Btwn(next(Stack), TopOfStack, l, null)
        ==> l == null || dom(Stack)[l]))
     && known(TopOfStack) && known(null) && knownF(next(Stack))
 }
@@ -120,12 +120,12 @@ function {:inline} Inv(TopOfStack: Loc, Stack: Heap) : (bool)
 
 // ---------- Primitives for manipulating ghost state
 
-procedure {:atomic} {:layer 1} AtomicReadTopOfStack() returns (v:Loc)
+procedure {:atomic} {:layer 1} AtomicReadTopOfStack() returns (v:Ref)
 { v := TopOfStack; assume known(v); }
 
-procedure {:yields} {:layer 0} {:refines "AtomicReadTopOfStack"} ReadTopOfStack() returns (v:Loc);
+procedure {:yields} {:layer 0} {:refines "AtomicReadTopOfStack"} ReadTopOfStack() returns (v:Ref);
 
-procedure {:right} {:layer 1} AtomicLoad(i:Loc) returns (v:Loc)
+procedure {:right} {:layer 1} AtomicLoad(i:Ref) returns (v:Ref)
 {
   assert dom(Stack)[i] || Used[i];
   if (dom(Stack)[i]) {
@@ -134,15 +134,15 @@ procedure {:right} {:layer 1} AtomicLoad(i:Loc) returns (v:Loc)
   }
 }
 
-procedure {:yields} {:layer 0} {:refines "AtomicLoad"} Load(i:Loc) returns (v:Loc);
+procedure {:yields} {:layer 0} {:refines "AtomicLoad"} Load(i:Ref) returns (v:Ref);
 
-procedure {:both} {:layer 1} AtomicStore({:linear_in "Node"} l_in:Heap, i:Loc, v:Loc) returns ({:linear "Node"} l_out:Heap)
+procedure {:both} {:layer 1} AtomicStore({:linear_in "Node"} l_in:Heap, i:Ref, v:Ref) returns ({:linear "Node"} l_out:Heap)
 { assert dom(l_in)[i]; l_out := Add(l_in, i, v);
   assume knownF(next(l_in)); }
 
-procedure {:yields} {:layer 0} {:refines "AtomicStore"} Store({:linear_in "Node"} l_in:Heap, i:Loc, v:Loc) returns ({:linear "Node"} l_out:Heap);
+procedure {:yields} {:layer 0} {:refines "AtomicStore"} Store({:linear_in "Node"} l_in:Heap, i:Ref, v:Ref) returns ({:linear "Node"} l_out:Heap);
 
-procedure {:atomic} {:layer 1} AtomicTransferToStack(oldVal: Loc, newVal: Loc, {:linear_in "Node"} l_in:Heap) returns (r: bool, {:linear "Node"} l_out:Heap)
+procedure {:atomic} {:layer 1} AtomicTransferToStack(oldVal: Ref, newVal: Ref, {:linear_in "Node"} l_in:Heap) returns (r: bool, {:linear "Node"} l_out:Heap)
 modifies TopOfStack, Stack;
 {
   assert dom(l_in)[newVal];
@@ -159,9 +159,9 @@ modifies TopOfStack, Stack;
   }
 }
 
-procedure {:yields} {:layer 0} {:refines "AtomicTransferToStack"} TransferToStack(oldVal: Loc, newVal: Loc, {:linear_in "Node"} l_in:Heap) returns (r: bool, {:linear "Node"} l_out:Heap);
+procedure {:yields} {:layer 0} {:refines "AtomicTransferToStack"} TransferToStack(oldVal: Ref, newVal: Ref, {:linear_in "Node"} l_in:Heap) returns (r: bool, {:linear "Node"} l_out:Heap);
 
-procedure {:atomic} {:layer 1} AtomicTransferFromStack(oldVal: Loc, newVal: Loc) returns (r: bool)
+procedure {:atomic} {:layer 1} AtomicTransferFromStack(oldVal: Ref, newVal: Ref) returns (r: bool)
 modifies TopOfStack, Used, Stack;
 {
   if (oldVal == TopOfStack) {
@@ -176,12 +176,12 @@ modifies TopOfStack, Used, Stack;
   }
 }
 
-procedure {:yields} {:layer 0} {:refines "AtomicTransferFromStack"} TransferFromStack(oldVal: Loc, newVal: Loc) returns (r: bool);
+procedure {:yields} {:layer 0} {:refines "AtomicTransferFromStack"} TransferFromStack(oldVal: Ref, newVal: Ref) returns (r: bool);
 
 
 // ---------- Stack methods:
 
-procedure {:atomic} {:layer 2} atomic_push(x: Loc, {:linear_in "Node"} x_Heap: Heap)
+procedure {:atomic} {:layer 2} atomic_push(x: Ref, {:linear_in "Node"} x_Heap: Heap)
 modifies Stack, TopOfStack;
 {
   Stack := Add(Stack, x, TopOfStack);
@@ -189,12 +189,12 @@ modifies Stack, TopOfStack;
   assume known(TopOfStack) && knownF(next(Stack));
 }
 
-procedure {:yields} {:layer 1} {:refines "atomic_push"} push(x: Loc, {:linear_in "Node"} x_Heap: Heap)
+procedure {:yields} {:layer 1} {:refines "atomic_push"} push(x: Ref, {:linear_in "Node"} x_Heap: Heap)
 requires {:layer 1} dom(x_Heap)[x];
 requires {:layer 1} Inv(TopOfStack, Stack);
 ensures {:layer 1} Inv(TopOfStack, Stack);
 {
-  var t: Loc;
+  var t: Ref;
   var g: bool;
   var {:linear "Node"} t_Heap: Heap;
 
@@ -227,16 +227,16 @@ ensures {:layer 1} Inv(TopOfStack, Stack);
   assert {:expand} {:layer 1} Inv(TopOfStack, Stack);
 }
 
-procedure {:atomic} {:layer 2} atomic_pop() returns (t: Loc)
+procedure {:atomic} {:layer 2} atomic_pop() returns (t: Ref)
 modifies Used, TopOfStack, Stack;
 { assume TopOfStack != null; t := TopOfStack; Used[t] := true; TopOfStack := next(Stack)[t]; Stack := Remove(Stack, t); }
 
-procedure {:yields} {:layer 1} {:refines "atomic_pop"} pop() returns (t: Loc)
+procedure {:yields} {:layer 1} {:refines "atomic_pop"} pop() returns (t: Ref)
 requires {:layer 1} Inv(TopOfStack, Stack);
 ensures {:layer 1} Inv(TopOfStack, Stack);
 {
   var g: bool;
-  var x: Loc;
+  var x: Ref;
 
   yield;
   assert {:layer 1} known(x) && known(t);
